좋아, lemma_is_distinct 증명, 거의 다 왔어!

src/common/Nemonuri.IndexMap.Unique.fst
@@ -1,47 +1,112 @@
 module Nemonuri.IndexMap.Unique
 
 open Nemonuri.IndexMap
-module Ui = Nemonuri.Unique.IntegerIntervals
+//module Ui = Nemonuri.Unique.IntegerIntervals
+module Lu = Nemonuri.LinearUnique
+module Ls = Nemonuri.LinearSearch
 module Cl = FStar.Classical
+open FStar.FunctionalExtensionality { (^->) }
+module F = FStar.FunctionalExtensionality
+
+let is_unique_in 
+  (#data_t:eqtype) (m:t data_t) (v:contained_data_t m) 
+  (imin:key_t m) (emax:key_or_count_t m{emax >= imin})
+  : Tot bool =
+  Lu.try_unique imin emax (equal_selection m v) |> Some?
 
 let unique_data_predicate (#data_t:eqtype) (m:t data_t) (v:contained_data_t m) : Tot bool =
-  (last_key m v) = (first_key m v)
+  is_unique_in m v 0 (count m)
+  //(last_key m v) = (first_key m v)
+
+let lemma_unique_data_predicate (#data_t:eqtype) (m:t data_t) (v:contained_data_t m) (witness:key_t m)
+  : Lemma 
+      (requires (equal_selection m v witness))
+      (ensures (unique_data_predicate m v) <==>
+               (Lu.predicate_is_linear_unique 0 (count m) (equal_selection m v) witness))
+  =
+  Lu.lemma_linear_unique 0 (count m) (equal_selection m v) witness
 
 type unique_data_t (#data_t:eqtype) (m:t data_t) = x:contained_data_t m{unique_data_predicate m x}
 
-let data_to_prop (#data_t:eqtype) (m:t data_t) (v:unique_data_t m) =
-  Ui.create_prop 
-    0 (count m) (equal_selection m v) (last_key m v) () () (lemma_contains_value m v)
-
-//let lemma_unique_data2 (#data_t:eqtype) (m:t data_t) (v:unique_data_t m)
-//  : Lemma ()
-
-let lemma_unique_data (#data_t:eqtype) (m:t data_t) (k:key_t m) (v:contained_data_t m)
-  : Lemma ((unique_data_predicate m v) ==> ((equal_selection m v k) <==> (last_key m v = k)))
-  =
-  match (unique_data_predicate m v) with | false -> () | true ->
-  assert (data_to_prop m v)
-  (*
-  let uk = last_key m v in
-  assert (~(equal_selection_restricted m v 0 (count m)));
-  assert (equal_selection_restricted m v (uk+1) (count m));
-  assert (equal_selection_restricted m v 0 uk);
-  assert (equal_selection m v uk)
-  *)
-  (*
-  let pl = (v = select m k) in
-  let pr = (last_key m v = k) in
-  let lemma_l_to_r' () : Lemma (requires pl) (ensures pr) =
-    assert (uk = k)
-  in
-  let lemma_r_to_l' () : Lemma (requires pr) (ensures pl) =
-     ()
-  in
-  Cl.move_requires lemma_l_to_r' ();
-  Cl.move_requires lemma_r_to_l' ()
-  *)
 
 let unique_key_predicate (#data_t:eqtype) (m:t data_t) (key:key_t m) : Tot bool =
   select m key |> unique_data_predicate m
 
+let lemma_unique_key_predicate (#data_t:eqtype) (m:t data_t) (key:key_t m)
+  : Lemma ((unique_key_predicate m key) <==> 
+           (Lu.predicate_is_linear_unique 0 (count m) (equal_selection_key m key) key))
+  =
+  let pl = (unique_key_predicate m key) in
+  let pr = (Lu.predicate_is_linear_unique 0 (count m) (equal_selection_key m key) key) in
+  let v = select m key in
+  let lemma_pl_to_pr' () : Lemma (pl ==> pr) =
+    assert (equal_selection m v key);
+    lemma_unique_data_predicate m v key
+  in
+  (* Note: 이게 왜 바로 증명이 되냐;; 나중에 내가 납득할 수 있도록 증명 해 봐야지. *)
+  let lemma_pr_to_pl' () : Lemma (pr ==> pl) =
+    //let f_t = (key_t m) ^-> Type0 in
+    //let tm1: f_t = F.on (key_t m) (equal_selection_key m key) in
+    //let tm2: f_t = F.on (key_t m) (equal_selection m v) in
+    //assert (F.feq #(key_t m) #(fun _ -> Type0) tm1 tm2);
+    //let tm3: f_t = F.on (key_t m) (Lu.predicate_is_linear_unique 0 (count m) tm1) in
+    //let tm4: f_t = F.on (key_t m) (Lu.predicate_is_linear_unique 0 (count m) tm2) in
+    //assert (F.feq #(key_t m) #(fun _ -> Type0) tm3 tm4);
+    //assert (Lu.predicate_is_linear_unique 0 (count m) tm2 key);
+    //assert (equal_selection m v key);
+    lemma_unique_data_predicate m v key
+  in
+  lemma_pl_to_pr' ();
+  lemma_pr_to_pl' ()
+
 type unique_key_t (#data_t:eqtype) (m:t data_t) = x:key_t m{unique_key_predicate m x}
+
+(*
+let is_max_selection_not_equal_in 
+  (#data_t:eqtype) (m:t data_t)
+  (imin:key_t m) (max:key_t m{max > imin})
+  : Tot bool =
+  let v = select m max in
+  Ls.desending_find imin max (equal_selection m v) |> None?
+
+let is_distinct (#data_t:eqtype) (m:t data_t)
+  : Tot bool =
+  match (count m) < 2 with | true -> true
+  | false -> 
+  let counterexample' (x:key_t m{x > 0}) : Tot bool =
+    not (is_max_selection_not_equal_in m 0 x)
+  in
+  Ls.ascending_find 1 (max_key m) counterexample' |> None?
+
+let lemma_is_distinct (#data_t:eqtype) (m:t data_t)
+  : Lemma ((is_distinct m) <==> (forall (x:key_t m). (unique_key_predicate m x)))
+  =
+  admit ()
+*)
+
+let map_is_distinct (#data_t:eqtype) (map:t data_t)
+  : Tot Type0 =
+  forall (x1:key_t map). 
+  forall (x2:key_t map{x2 < x1}). 
+    ~(equal_selection_key map x1 x2)
+
+//let map_is_distinct
+
+
+let lemma_is_distinct (#data_t:eqtype) (m:t data_t)
+  : Lemma ((map_is_distinct m) <==> (forall (x:key_t m). (unique_key_predicate m x)))
+  =
+  let pl = (map_is_distinct m) in
+  let pr = (forall (x:key_t m). (unique_key_predicate m x)) in
+  let pr1 = (forall (x:key_t m). (Lu.predicate_is_linear_unique 0 (count m) (equal_selection_key m x) x)) in
+  let pl1 = (forall (x1 x2:key_t m). (x1 <> x2) ==> ~(equal_selection_key m x1 x2)) in
+
+  let lemma_pr_pr1' () : Lemma (pr <==> pr1) =
+    Cl.forall_intro (lemma_unique_key_predicate m)
+  in
+  let lemma_pl_pl1' () : Lemma (pl <==> pl1) =
+    admit ()
+  in
+
+  lemma_pr_pr1' ();
+  lemma_pl_pl1' ()
